src/Layer1to2Refinement.v
@@ -1,53 +1,143 @@
-Require Import Primitives Layer1 BlockAllocator Layer2.
+Require Import Primitives Layer1 BlockAllocator.
+Require Import Layer2 SimulationLayer.
+Require Import FunctionalExtensionality Omega.
 
 Section Layer1to2Refinement.
   
-  Fixpoint prog2to1 {T} (p1: Layer2.prog T) : Layer1.prog T :=
+  Fixpoint compile {T} (p1: Layer2.prog T) : Layer1.prog T :=
     match p1 with
     | Read a => read a
     | Write a v => write a v
     | Alloc v => alloc v
     | Free a => free a
     | Ret v => Layer1.Ret v
-    | Bind px py => Layer1.Bind (prog2to1 px) (fun x => prog2to1 (py x))
+    | Bind px py => Layer1.Bind (compile px) (fun x => compile (py x))
     end.
   
-  Fixpoint oracle_matches {T} (st1: Layer1.state) (o2: Layer2.oracle) (p: Layer2.prog T) :=
+  Fixpoint oracle_matches T (d1: Layer1.state) (p: Layer2.prog T)  (o1: oracle Layer1.token) (o2: oracle Layer2.token) :=
     match p with
     | Alloc v =>
-      forall o1' d1',
-        (Layer1.exec st1 (prog2to1 (Alloc v)) (Crashed (o1', d1')) ->
+      forall d1',
+        (Layer1.exec o1 d1 (compile (Alloc v)) (Crashed d1') ->
          o2 = [Crash]) /\
-        (forall r, Layer1.exec st1 (prog2to1 (Alloc v)) (Finished (o1', d1') r) ->
+        (forall r, Layer1.exec o1 d1 (compile (Alloc v)) (Finished d1' r) ->
          match r with
          | Some a =>
            o2 = [BlockNum a]
          | None =>
            o2 = [DiskFull]
          end)
-    | Bind p1 p2 =>
-       forall o1' d1',
-        (Layer1.exec st1 (prog2to1 p1) (Crashed (o1', d1')) ->
-         o2 = [Crash]) /\
-        (forall r o2' o2'',
-            Layer1.exec st1 (prog2to1 p1) (Finished (o1', d1') r) ->
-            oracle_matches st1 o2' p1 ->
-            oracle_matches (o1', d1') o2'' (p2 r) ->
-            o2 = o2'++o2'')
+    | @Bind T1 T2 p1 p2 =>
+       forall d1',
+        (Layer1.exec o1 d1 (compile p1) (Crashed d1') ->
+         oracle_matches T1 d1 p1 o1 o2) /\
+        (forall r o1' o1'' o2' o2'',
+           o1 = o1'++o1'' ->
+           o2 = o2'++o2'' ->
+           Layer1.exec o1' d1 (compile p1) (Finished d1' r) ->
+           oracle_matches T1 d1 p1 o1' o2' /\
+           oracle_matches T2 d1' (p2 r) o1'' o2'')
     | _ =>
-      forall o1' d1',
-        (Layer1.exec st1 (prog2to1 p) (Crashed (o1', d1')) ->
+      forall d1',
+        (Layer1.exec o1 d1 (compile p) (Crashed d1') ->
          o2 = [Crash]) /\
-        (forall r, Layer1.exec st1 (prog2to1 p) (Finished (o1', d1') r) ->
+        (forall r, Layer1.exec o1 d1 (compile p) (Finished d1' r) ->
          o2 = [Cont])
     end.
- 
-  Check oracle_matches.
 
-  Definition refines_to {T} st1 st2 (p: Layer2.prog T) :=
-    let '(o1, d1) := st1 in
-    let '(o2, d2) := st2 in
-    rep d2 d1 /\
-    oracle_matches st1 o2 p.
+  Definition refines_to d1 d2 :=
+    rep d2 d1.
 
+  Definition compiles_to T p2 p1 :=
+    p1 = @compile T p2.
+
+  Definition low := Build_LTS Layer1.token Layer1.state Layer1.prog Layer1.exec.
+
+  Definition high := Build_LTS Layer2.token Layer2.state Layer2.prog Layer2.exec.
+
+  Lemma rep_eq:
+    forall d s1 s2,
+      rep s1 d ->
+      rep s2 d ->
+      s1 = s2.
+  Proof.
+    intros.
+    extensionality k.
+    unfold rep in *.
+    destruct_lift H. destruct_lift H0.
+    eapply_fresh ptsto_valid in H.
+    eapply_fresh ptsto_valid in H0; cleanup.
+    destruct_fresh (nth k (bits (value_to_bits dummy2)) 0).
+    rewrite H4, H6; eauto.
+    destruct (value_to_bits dummy2); simpl in *.
+    unfold valid_bitlist in *; cleanup.
+    destruct (nth_in_or_default k bits 0); [|cleanup; omega].
+    apply H2 in i; cleanup.
+    destruct n; cleanup; try omega.
+    specialize (H3 _ D).
+    specialize (H5 _ D); cleanup; eauto.
+  Qed.
   
+  Theorem sbs :
+    forall valid_h valid_op_h,
+    StrongBisimulation low high
+                       (refines_to_valid refines_to valid_h)
+                       (compiles_to_valid valid_op_h compiles_to)
+                       valid_h
+                       valid_op_h
+                       compiles_to refines_to
+                       oracle_matches.
+  Proof.
+    unfold refines_to_valid, refines_to,
+    compiles_to_valid, compiles_to, oracle_matches; intros.
+    constructor.
+    intros T p1 p2.
+    generalize dependent p1.
+    induction p2; intros.
+    - (* Read *)
+      simpl in *; cleanup.
+      split.
+      + (* Low to High *)
+        intros.
+        eapply_fresh read_ok in H0.
+        2: instantiate (2:= emp); pred_apply; cancel.
+        split_ors; cleanup.
+        * (* Finished *)
+          destruct_lifts.
+          specialize (H5 x0); cleanup.
+          eexists.
+          split.
+          econstructor; eauto.
+          simpl in *.
+          repeat split; eauto.
+          intuition (cleanup; eauto).
+          unfold rep in *.
+          destruct_lift H7.
+          erewrite H13; eauto; simpl.
+          apply nth_overflow; simpl.
+          destruct (value_to_bits dummy); simpl.
+          unfold valid_bitlist in *; cleanup; eauto.
+          intros.
+          erewrite rep_eq; eauto.
+
+        * (* Crashed *)
+          destruct_lifts.
+          specialize (H5 x0); cleanup.
+          eexists.
+          split.
+          eapply ExecOpCrash; eauto.
+          intros; intuition.
+          inversion H9.
+          simpl in *.
+          repeat split; eauto.
+          intuition (cleanup; eauto).
+          erewrite rep_eq; eauto.
+
+      + (*High to low*)
+        intros.
+        inversion H0; sigT_eq.
+        (* Total correctness needed 
+           to show that such execution exists *)
+  Abort.
+
+End Layer1to2Refinement.
