src/SimulationLayer.v
@@ -1,25 +1,4 @@
-Require Import List CommonAutomation.
-
-Inductive Result {State T: Type} :=
-| Finished : State -> T -> @Result State T
-| Crashed : State -> @Result State T.
-
-Definition extract_state {State T} (res: @Result State T) :=
-  match res with
-  | Finished s _ | Crashed s => s
-  end.
-
-Definition extract_ret {State T} def (res: @Result State T) :=
-  match res with
-  | Finished _ r => r
-  | Crashed _ => def
-  end.
-
-Definition result_same {State1 State2 T1 T2} (res1: @Result State1 T1) (res2: @Result State2 T2) :=
-  match res1, res2 with
-  | Finished _ _, Finished _ _ | Crashed _, Crashed _ => True
-  | _, _ => False
-  end.
+Require Import List CommonAutomation Simulation.
 
 Lemma result_same_transitive:
   forall State1 State2 State3 T1 T2 T3
@@ -47,9 +26,10 @@ Qed.
 
 Record LTS :=
   {
+    Token : Type;
     State : Type;
     Op : Type -> Type;
-    transition : forall T, State -> Op T -> @Result State T -> Prop;
+    transition : forall T, list Token -> State -> Op T -> @Result State T -> Prop;
   }.
 
 Definition refines_to_related {T1 T2} refines_to (R: T2 -> T2 -> Prop) (st1 st2: T1) :=
@@ -63,26 +43,52 @@ Definition refines_to_valid {T1 T2} (refines_to: T1 -> T2 -> Prop) (valid2: T2 -
     refines_to st1 st2 ->
     valid2 st2.
 
+Definition oracle_refines_to_valid
+           {State1 State2 Oracle1 Oracle2: Type} {Op1 Op2: Type -> Type}
+           (oracle_refines_to: forall T, State1 -> Op2 T -> Oracle1 -> Oracle2 -> Prop)
+           (refines_to: State1 -> State2 -> Prop)
+           (compiles_to: forall T, Op2 T -> Op1 T -> Prop)
+           (valid_oracle2: forall T, Oracle2 -> State2 -> Op2 T -> Prop)
+           T (o1: Oracle1) (st1: State1) (p1: Op1 T) :=
+  forall st2 p2,
+    refines_to st1 st2 ->
+    compiles_to T p2 p1 ->
+    exists o2, oracle_refines_to T st1 p2 o1 o2 /\
+    valid_oracle2 T o2 st2 p2.
+
 Definition compiles_to_valid {Op1 Op2: Type -> Type}
            (valid_op2: forall T, Op2 T -> Prop)
            (compiles_to: forall T, Op2 T -> Op1 T -> Prop)  T (o1: Op1 T) :=
   exists o2, compiles_to T o2 o1 /\ valid_op2 T o2.
 
+Definition oracle_equal_with_respect_to
+           {State Oracle1 Oracle2: Type} {Op: Type -> Type}
+           (related: State -> State -> Prop)
+           (oracle_refines_to: forall T, State -> Op T -> Oracle1 -> Oracle2 -> Prop):=
+  forall T o1 o2 o2' st1 st2 p,
+    oracle_refines_to T st1 p o1 o2 ->
+    oracle_refines_to T st2 p o1 o2' ->
+    related st1 st2 ->
+    o2 = o2'.
+
 
 Record SelfSimulation (lts: LTS)
        (valid_state: State lts -> Prop)
        (valid_op: forall T, Op lts T -> Prop)
+       (valid_oracle: forall T, list (Token lts) -> State lts -> Op lts T -> Prop)
        (R: State lts -> State lts -> Prop) :=
   {
     self_simulation_correct:
-      forall T o s1 s1' s2,
+      forall T o p s1 s1' s2,
         valid_state s1 ->
         valid_state s2 ->
-        valid_op T o ->
-        (transition lts) T s1 o s1' ->
+        valid_op T p ->
+        valid_oracle T o s1 p ->
+        valid_oracle T o s2 p ->
+        (transition lts) T o s1 p s1' ->
         R s1 s2 ->
         exists s2',
-          (transition lts) T s2 o s2' /\
+          (transition lts) T o s2 p s2' /\
           result_same s1' s2' /\
           R (extract_state s1') (extract_state s2') /\
           (forall def, extract_ret def s1' = extract_ret def s2') /\
@@ -97,31 +103,35 @@ Record StrongBisimulation
        (valid_state2 : State lts2 -> Prop)
        (valid_op2: forall T, Op lts2 T -> Prop)
        (compiles_to: forall T, Op lts2 T -> Op lts1 T -> Prop)
-       (refines_to: State lts1 -> State lts2 -> Prop):=
+       (refines_to: State lts1 -> State lts2 -> Prop)
+       (oracle_refines_to: forall T, State lts1 -> Op lts2 T -> list (Token lts1) -> list (Token lts2) -> Prop)
+  :=
   {
     strong_bisimulation_correct:
-      (forall T o1 o2 s1 s2,
+      (forall T p1 p2 o1 o2 s1 s2,
           valid_state1 s1 ->
-          valid_op1 T o1 ->
+          valid_op1 T p1 ->
           
           valid_state2 s2 ->
-          valid_op2 T o2 ->
+          valid_op2 T p2 ->
           
           refines_to s1 s2 ->
-          compiles_to T o2 o1 ->
+          compiles_to T p2 p1 ->
+          
+          oracle_refines_to T s1 p2 o1 o2 ->
           
           (forall s1',
-              (transition lts1) T s1 o1 s1' ->
+              (transition lts1) T o1 s1 p1 s1' ->
               exists s2',
-                (transition lts2) T s2 o2 s2' /\
+                (transition lts2) T o2 s2 p2 s2' /\
                 result_same s1' s2' /\
                 refines_to (extract_state s1') (extract_state s2') /\
                 (forall def, extract_ret def s1' = extract_ret def s2') /\
                 valid_state1 (extract_state s1') /\ valid_state2 (extract_state s2')) /\
           (forall s2',
-              (transition lts2) T s2 o2 s2' ->
+              (transition lts2) T o2 s2 p2 s2' ->
               exists s1',
-                (transition lts1) T s1 o1 s1' /\
+                (transition lts1) T o1 s1 p1 s1' /\
                 result_same s1' s2' /\
                 refines_to (extract_state s1') (extract_state s2') /\
                 (forall def, extract_ret def s1' = extract_ret def s2')/\
@@ -129,41 +139,121 @@ Record StrongBisimulation
   }.
 
 Theorem transfer_high_to_low :
-  forall low high eqv_h refines_to compiles_to valid_h valid_op_h,
-    SelfSimulation high
-                   valid_h
-                   valid_op_h
-                   eqv_h ->
-    StrongBisimulation low high
-                       (refines_to_valid refines_to valid_h)
-                       (compiles_to_valid valid_op_h compiles_to)
-                       valid_h
-                       valid_op_h
-                       compiles_to refines_to ->
-    SelfSimulation low
-                   (refines_to_valid refines_to valid_h)
-                   (compiles_to_valid  valid_op_h compiles_to)
-                   (refines_to_related refines_to eqv_h).
+  forall low high
+
+    eqv_h
+    refines_to
+    compiles_to
+    oracle_refines_to
+
+    valid_h
+    valid_op_h
+    valid_oracle_h,
+    
+    SelfSimulation
+      high
+      valid_h
+      valid_op_h
+      valid_oracle_h
+      eqv_h ->
+    
+    StrongBisimulation
+      low
+      high
+      (refines_to_valid
+         refines_to
+         valid_h)
+      (compiles_to_valid
+         valid_op_h
+         compiles_to)
+      valid_h
+      valid_op_h
+      compiles_to
+      refines_to
+      oracle_refines_to ->
+
+    oracle_equal_with_respect_to
+      (refines_to_related
+         refines_to
+         eqv_h)
+      oracle_refines_to ->
+    
+    SelfSimulation
+      low
+      (refines_to_valid
+         refines_to
+         valid_h)
+      (compiles_to_valid
+         valid_op_h
+         compiles_to)
+      (oracle_refines_to_valid
+         oracle_refines_to
+         refines_to
+         compiles_to
+         valid_oracle_h)
+      (refines_to_related
+         refines_to
+         eqv_h).
 Proof.
-  unfold refines_to_related, compiles_to_valid; intros.
+  unfold refines_to_related, compiles_to_valid, oracle_refines_to_valid, oracle_equal_with_respect_to; intros.
   destruct H, H0.
   rename self_simulation_correct0 into self_simulation_correct.
   rename strong_bisimulation_correct0 into strong_bisimulation_correct.
   
   eapply Build_SelfSimulation;  intros; cleanup.
-  eapply strong_bisimulation_correct in H3 as Hx; eauto; cleanup.
-  eapply H7 in H2; cleanup.
-  clear H7 H8.
+  repeat match goal with
+    | [H: forall (st2 : State high) (p2 : Op high T), _ |- _] =>
+      edestruct H; eauto; cleanup; clear H
+  end.
+  eapply_fresh H1 in H10; eauto; cleanup.
 
-  eapply_fresh H in H3.
-  eapply_fresh H0 in H4.
-  eapply self_simulation_correct in H2; eauto; cleanup.  
+  match goal with
+  | [H: refines_to s1 _ |- _] =>
+    eapply_fresh strong_bisimulation_correct in H; eauto; cleanup
+  end.
+
+  match goal with
+    | [H: forall _, transition low _ _ _ _ _ -> _,
+       H0: transition low _ _ _ _ _,
+       H1: forall _, transition high _ _ _ _ _ -> _ |- _] =>
+      eapply H in H0; cleanup; clear H H1
+  end.
+
+  match goal with
+  | [H: refines_to_valid _ _ ?s,
+     H0: refines_to ?s _,
+     H1: refines_to_valid _ _ ?t,
+     H2: refines_to ?t _ |- _] =>
+    eapply_fresh H in H0;
+      eapply_fresh H1 in H2; cleanup
+  end.
+
+  match goal with
+    | [H: transition high _ _ _ _ _ |- _] =>
+      eapply self_simulation_correct in H; eauto; cleanup
+  end.
+
+  match goal with
+  | [H: transition high _ _ ?x2 _ _,
+     H0: refines_to ?s1 ?x1,
+     H1: refines_to ?s2 ?x2,      
+     H2: refines_to_valid _ _ ?s2 |- _] =>
+      eapply strong_bisimulation_correct in H1; eauto; cleanup
+  end.
   
-  eapply_fresh strong_bisimulation_correct in H4; eauto; cleanup.
-  apply H17 in H2; cleanup.
-  clear H15 H17.
+  match goal with
+    | [H: forall _, transition low _ _ _ _ _ -> _,
+       H0: transition high _ _ _ _ _,
+       H1: forall _, transition high _ _ _ _ _ -> _ |- _] =>
+      eapply H1 in H0; cleanup; clear H H1
+  end.
+
   eexists; intuition eauto.
   do 2 (eapply result_same_transitive; eauto).
   apply result_same_symmetric; auto.
-  rewrite H11, H20; auto.  
+  
+  repeat match goal with
+  | [H: forall _, extract_ret _ ?a = _ |- extract_ret _ ?a = _] =>
+    rewrite H; auto
+  end.
 Qed.
