src/ProgAuto.v
@@ -9,32 +9,36 @@ Ltac invert_exec'' H :=
 
 Ltac invert_exec' :=
   match goal with
-  | [ H: exec _ (Ret _) _ |- _ ] =>
-    invert_exec'' H
-  | [ H: exec _ (Read _) _ |- _ ] =>
-    invert_exec'' H
-  | [ H: exec _ (Write _ _) _ |- _ ] =>
-    invert_exec'' H
+  | [ H: exec _ _ ?p _ |- _ ] =>
+    match p with
+    | Bind _ _ => idtac
+    | Read _ => invert_exec'' H
+    | Write _ _ => invert_exec'' H
+    | Ret _ => invert_exec'' H
+    end
   end.
 
 Lemma bind_sep:
-  forall T T' st (p1: prog T) (p2: T -> prog T') ret,
-    exec st (Bind p1 p2) ret ->
+  forall T T' o d (p1: prog T) (p2: T -> prog T') ret,
+    exec o d (Bind p1 p2) ret ->
     match ret with
-    | Finished st' r =>
-    (exists r1 st1,
-       exec st p1 (Finished st1 r1) /\
-       exec st1 (p2 r1) ret)
-  | Crashed st' =>
-    (exec st p1 (Crashed st') \/
-     (exists r1 st1,
-        exec st p1 (Finished st1 r1) /\
-        exec st1 (p2 r1) ret ))
-  | Failed st' =>
-    (exec st p1 (Failed st') \/
-     (exists r1 st1,
-        exec st p1 (Finished st1 r1) /\
-        exec st1 (p2 r1) ret ))
+    | Finished d' r =>
+    (exists o1 o2 d1 r1,
+       exec o1 d p1 (Finished d1 r1) /\
+       exec o2 d1 (p2 r1) ret /\
+       o = o1++o2)
+  | Crashed d' =>
+    (exec o d p1 (Crashed d') \/
+     (exists o1 o2 d1 r1,
+        exec o1 d p1 (Finished d1 r1) /\
+        exec o2 d1 (p2 r1) ret /\
+        o = o1++o2))
+  | Failed d' =>
+    (exec o d p1 (Failed d') \/
+     (exists o1 o2 d1 r1,
+        exec o1 d p1 (Finished d1 r1) /\
+        exec o2 d1 (p2 r1) ret /\
+        o = o1++o2))
     end.
 Proof.
   intros.
@@ -47,16 +51,16 @@ Qed.
 
 Ltac invert_exec :=
   match goal with
-  |[H : exec _ (Bind _ _) _ |- _ ] =>
+  |[H : exec _ _ (Bind _ _) _ |- _ ] =>
    apply bind_sep in H; repeat cleanup
-  |[H : exec _ _ _ |- _ ] =>
+  |[H : exec _ _ _ _ |- _ ] =>
    invert_exec'
   end.
 
 
   Definition prog_equiv T : prog T -> prog T -> Prop :=
-    fun p1 p2 => forall st out,
-        exec st p1 out <-> exec st p2 out.
+    fun p1 p2 => forall o d out,
+        exec o d p1 out <-> exec o d p2 out.
 
   Arguments prog_equiv {T} _ _.
 
@@ -67,6 +71,7 @@ Ltac invert_exec :=
   Proof.
     split; intros.
     - repeat invert_exec; cleanup.
+      rewrite <- app_assoc.
       repeat econstructor; eauto.
 
       split_ors.
@@ -76,6 +81,7 @@ Ltac invert_exec :=
       econstructor; eauto.
       eapply ExecBindCrash; eauto.
       invert_exec.
+      rewrite <- app_assoc.
       repeat econstructor; eauto.
 
       split_ors.
@@ -85,9 +91,11 @@ Ltac invert_exec :=
       econstructor; eauto.
       eapply ExecBindFail; eauto.
       invert_exec.
+      rewrite <- app_assoc.
       repeat econstructor; eauto.
     
     - repeat invert_exec; cleanup.
+      rewrite app_assoc.
       repeat (eapply ExecBind; eauto).
       
       split_ors.
@@ -97,6 +105,7 @@ Ltac invert_exec :=
       split_ors.
       eapply ExecBindCrash; eauto.
       econstructor; eauto.
+      rewrite app_assoc.
       repeat econstructor; eauto.
 
       split_ors.
@@ -106,5 +115,6 @@ Ltac invert_exec :=
       split_ors.
       eapply ExecBindFail; eauto.
       econstructor; eauto.
+      rewrite app_assoc.
       repeat econstructor; eauto.
   Qed.
